Merge, and some progress towards un-lining the push and adjustWeight functions of the PQ

sample_mark/priorityqueue.h
@@ -1,6 +1,10 @@
 
 #define SIZE 8
 
+void push (int vertex, int weight, int pq[SIZE]);
+
 int popMin (int pq[SIZE]);
+
+void adjustWeight (int vertex, int newWeight, int pq[SIZE]);
 
 int pq_emp (int pq[SIZE]);
