sample_mark/env_dijkstra_arr.v
@@ -1,10 +1,11 @@
 Require Export VST.floyd.proofauto.
 Require Export RamifyCoq.floyd_ext.closed_lemmas.
-(* Require Export RamifyCoq.sample_mark.priorityqueue. *)
 Require Export RamifyCoq.sample_mark.dijkstra.
 
 Instance CompSpecs : compspecs. Proof. make_compspecs prog. Defined.
 Definition Vprog : varspecs. mk_varspecs prog. Defined.
-
 Global Existing Instance CompSpecs.
+
 Definition vertex_type := tint.
+
+Locate _pq.
